[CFG] start removing edges of CFG

attic/CFG.thy
@@ -28,20 +28,12 @@ type_synonym pos_inst = "position * inst"
 type_synonym vert = "pos_inst list * tblock"
 type_synonym vertex = "int * vert"
 type_synonym vertices = "vertex list"
-type_synonym edge = "int * (int option)"
-type_synonym edges = "int \<Rightarrow> edge option"
 
 type_synonym stack_value = "w256 option"
-
-type_synonym edges_status = "string option"
-typ "stack_value list + string"
-type_synonym edges_return = "edges * edges_status"
 
 record cfg =
 cfg_indexes :: "int list"
 cfg_blocks :: "int \<Rightarrow> vert option"
-cfg_edges :: "edges"
-cfg_status :: "edges_status"
 
 (* Auxiliary functions *)
 
@@ -69,29 +61,8 @@ fun good_dest :: "int \<Rightarrow> vertices \<Rightarrow> bool" where
 | "good_dest m ((n,[],_)#l) = good_dest m l"
 | "good_dest m ((n,(_,i)#inst,_)#l) = (if m = n then (i = Pc JUMPDEST) else good_dest m l )"
 
-definition not_complete :: "edges_return \<Rightarrow> char list \<Rightarrow> edges_return " where
-  "not_complete res debug= (fst res, Some debug)"
-
-definition update_edges :: "edges_return \<Rightarrow> int \<Rightarrow> edge \<Rightarrow> edges_return" where
-"update_edges e i v = ((fst e)(i:= Some v), snd e)"
-
-definition concat_map :: "int \<Rightarrow> edge \<Rightarrow> edges_return \<Rightarrow> edges_return \<Rightarrow> edges_return" where
- "concat_map n v m1 m2 = 
-  ((fst m1 ++ fst m2)(n:= Some v),(case (snd m1, snd m2) of
-    (Some str1, _) \<Rightarrow> Some str1
-   |(_, Some str1) \<Rightarrow> Some str1
-   |_ \<Rightarrow> None
-))"
-
 definition extract_indexes :: "vertices \<Rightarrow> int list" where
 "extract_indexes xs = map v_ind xs"
-
-fun print_edges_aux ::"int list \<Rightarrow> edges \<Rightarrow> (int * edge) list" where
-"print_edges_aux [] e = []"
-| "print_edges_aux (n#q) e = (case e n of None \<Rightarrow> print_edges_aux q e | Some i \<Rightarrow> (n,i) # (print_edges_aux q e))"
-
-abbreviation print_edges :: "vertices \<Rightarrow> edges_return \<Rightarrow> (int * edge) list" where
-"print_edges v e == print_edges_aux (extract_indexes v) (fst e)"
 
 (* Stack manipulations *)
 
@@ -132,69 +103,12 @@ fun aux_basic_block :: "inst list \<Rightarrow> int \<Rightarrow> int \<Rightarr
 definition build_basic_blocks :: "inst list \<Rightarrow> vertices" where
 "build_basic_blocks prog == aux_basic_block prog 0 0 []"
 
-(* Read a block and simulate stack operations - only store push values *)
-fun edge_one_block :: "tblock \<Rightarrow> pos_inst list \<Rightarrow> stack_value list \<Rightarrow> (stack_value list + string)" where
-  "edge_one_block Next [] st = Inl st"
-| "edge_one_block No [] st = Inl st"
-| "edge_one_block Jump [] [] = Inr ''JUMP : Empty stack''"
-| "edge_one_block Jump [] (a#st) = (case a of
-      Some add \<Rightarrow> Inl (a#st)
-    | None \<Rightarrow> Inr ''JUMP : Data on top of the stack'')"
-| "edge_one_block Jumpi [] [] = Inr ''JUMPI : Empty stack''"
-| "edge_one_block Jumpi [] [a] = Inr ''JUMPI : Just 1 elet on stack''"
-| "edge_one_block Jumpi [] (a#b#st) = (case a of
-      Some add \<Rightarrow> Inl (a#b#st)
-    | None \<Rightarrow> Inr ''JUMPI : Data on top of the stack'')"
-| "edge_one_block t ((_,(Stack (PUSH_N data)))#bl) st = 
-    edge_one_block t bl ((Some (Word.word_rcat (constant_mark data)))#st)"
-| "edge_one_block t ((_,Swap i)#bl) st = (case list_swap (unat i + 1) st of
-    None \<Rightarrow> Inr ''Swap : stack too small''
-  | Some st \<Rightarrow> edge_one_block t bl st)"
-| "edge_one_block t ((_,Dup i)#bl) st = ( (case index st (unat i) of
-    None => Inr ''Dup : stack too small''
-  | Some duplicated => edge_one_block t bl (duplicated # st)))"
-| "edge_one_block t ((_,i)#bl) st = (let st_nb= (inst_stack_numbers i) in
-    (if (nat (fst st_nb))>length st
-     then Inr ''Stack too small''
-     else edge_one_block t bl ((replicate (nat (snd st_nb)) None)@(drop (nat (fst st_nb)) st))))"
-
-(* Compute the edges of a block *)
-fun edges_blocks :: "int list \<Rightarrow> int \<Rightarrow> stack_value list \<Rightarrow> vertices \<Rightarrow> edges_return " where
-"edges_blocks to_do n st vertices = 
-  (if n \<in> set to_do then
-   (case find (find_block n) vertices of
-      None \<Rightarrow> (Map.empty, Some ''Block not found'')
-    | Some bl \<Rightarrow> (let new_to_do = removeAll n to_do in
-      (case edge_one_block (v_ty bl) (v_insts bl) st of
-        Inr str \<Rightarrow> (Map.empty, Some str)
-       |Inl st \<Rightarrow> (case v_ty bl of
-          No \<Rightarrow> (Map.empty, None)
-        | Next \<Rightarrow> let m = next_i vertices n in
-           update_edges (edges_blocks new_to_do m st vertices) n (m, None)
-        | Jump \<Rightarrow> (case st of 
-            (Some a)#sta \<Rightarrow> 
-            (if good_dest (uint a) vertices
-            then update_edges (edges_blocks new_to_do (uint a) sta vertices) n (uint a, None)
-            else (Map.empty, Some ''Bad destination for JUMP''))
-            |_ \<Rightarrow> (Map.empty, Some ''Bad stack for JUMP''))
-        | Jumpi \<Rightarrow> (case st of
-            (Some a)#b#sta \<Rightarrow> (let m = next_i vertices n in
-              (if good_dest (uint a) vertices
-              then concat_map n ((uint a), Some m) (edges_blocks new_to_do m sta vertices) (edges_blocks new_to_do (uint a) sta vertices)
-              else (fst (update_edges (edges_blocks new_to_do m sta vertices) n ((uint a), Some m)), Some ''Bad destination for JUMPI'')))
-            | _ \<Rightarrow> (Map.empty, Some ''Bad stack for JUMPI''))
-  ))))
-  else (Map.empty, None))"
-
 definition build_cfg :: "inst list \<Rightarrow> cfg" where
 "build_cfg prog = (let blocks = build_basic_blocks prog in
 (let ind = (extract_indexes blocks) in
-(let edges = edges_blocks ind 0 [] blocks in
 (|cfg_indexes = ind,
-  cfg_blocks = map_of blocks,
-  cfg_edges = fst edges,
-  cfg_status = snd edges |)
-)))"
+  cfg_blocks = map_of blocks|)
+))"
 
 (* Verification *)
 
@@ -292,29 +206,20 @@ definition last_no::"pos_inst list \<Rightarrow> bool" where
 "last_no insts == snd (last insts) \<in> {Misc STOP, Misc RETURN, Misc SUICIDE}"
 
 definition wf_cfg:: "cfg \<Rightarrow> bool" where
-"wf_cfg c == cfg_status c = None \<longrightarrow>
-(\<forall>n insts ty m i j.
+"wf_cfg c == 
+(\<forall>n insts ty i.
 (cfg_blocks c n = Some (insts, ty) \<longrightarrow>
 	n \<in> set (cfg_indexes c) \<and> reg_vertex (n, insts, ty) \<and>
   insts \<noteq> [] \<and> (fst (hd insts) = n) \<and> seq_block insts \<and>
   0 < n \<and> n < 2 ^ 256) \<and>
-(cfg_blocks c n = Some (insts, Next) \<longrightarrow>
-	cfg_edges c n = Some (m, None) \<longrightarrow>
-	(m = n + inst_size_list insts)) \<and>
 (cfg_blocks c n = Some (insts, Jump) \<longrightarrow>
 	i = n + inst_size_list insts \<longrightarrow>
-	cfg_edges c n = Some (m, None) \<longrightarrow>
-	(program_content (program_from_cfg c) m = Some (Pc JUMPDEST) \<and>
-	 program_content (program_from_cfg c) i = Some (Pc JUMP))) \<and>
+	program_content (program_from_cfg c) i = Some (Pc JUMP)) \<and>
 (cfg_blocks c n = Some (insts, Jumpi) \<longrightarrow>
 	i = n + inst_size_list insts \<longrightarrow>
-	cfg_edges c n = Some (m, Some j) \<longrightarrow>
-	(program_content (program_from_cfg c) m = Some (Pc JUMPDEST) \<and>
-	 program_content (program_from_cfg c) i = Some (Pc JUMPI) \<and>
-	 j = i + 1)) \<and>
+	program_content (program_from_cfg c) i = Some (Pc JUMPI)) \<and>
 (cfg_blocks c n = Some (insts, No) \<longrightarrow>
-	(cfg_edges c n = None \<and>
-   last_no insts))
+   last_no insts)
 )"
 
 end
